theories/SpecNotations.v
@@ -9,13 +9,13 @@ Infix "*" := t_prod.
 
 Notation "'η'" := (eta) (at level 0).
 
-Notation "G ⊢ v ⇐ t" := (Jv G v t) (at level 90).
-Notation "G ⊢ V ⇒ t" := (JV G V t) (at level 90).
+Notation "X @ G ⊢ v ⇐ t" := (Jv X G v t) (at level 90).
+Notation "X @ G ⊢ V ⇒ t" := (JV X G V t) (at level 90).
 
-Notation "ρ ⊢ v ⇓ v'" := (bigv ρ v v') (at level 90).
+(* Notation "ρ ⊢ v ⇓ v'" := (bigv ρ v v') (at level 90). *)
 (* Notation "ρ ⊢ V ⇓ v'" := (bigv ρ V v') (at level 90). *)
 
-Notation "D ⊢ E ⊠ D'" := (sE D E D') (at level 90).
+(* Notation "D ⊢ E ⊠ D'" := (sE D E D') (at level 90). *)
 
 Infix "|-" := P_with (at level 30).
 
